Write down footprints

ind/DListLowInd.fst
@@ -106,6 +106,62 @@ let rec nodelist_contained_b (#t:Type) (h0:heap) (nl:nodelist t) : GTot Type0 =
 
 (* piece containment is given by its ghostly connections *)
 
+/// Footprints
+
+let node_fp_f (#t:Type) (n:node t) : GTot Mod.loc =
+  Mod.loc_buffer n.flink
+let node_fp_b (#t:Type) (n:node t) : GTot Mod.loc =
+  Mod.loc_buffer n.blink
+
+let rec nodelist_fp0 (#t:Type) (n:nodelist t) : GTot Mod.loc =
+  match n with
+  | [] -> Mod.loc_none
+  | n :: ns -> Mod.loc_union (Mod.loc_buffer n) (nodelist_fp0 ns)
+let rec nodelist_fp_f (#t:Type) (h0:heap) (n:nodelist t) : GTot Mod.loc =
+  match n with
+  | [] -> Mod.loc_none
+  | n :: ns -> Mod.loc_union (Mod.loc_buffer (n@h0).flink) (nodelist_fp_f h0 ns)
+let rec nodelist_fp_b (#t:Type) (h0:heap) (n:nodelist t) : GTot Mod.loc =
+  match n with
+  | [] -> Mod.loc_none
+  | n :: ns -> Mod.loc_union (Mod.loc_buffer (n@h0).blink) (nodelist_fp_b h0 ns)
+
+let dll_fp0 (#t:Type) (d:dll t) : GTot Mod.loc =
+  Mod.loc_union // ghostly connections should give us this union for
+                // free, but still useful to have
+    (Mod.loc_union (Mod.loc_buffer d.lhead) (Mod.loc_buffer d.ltail))
+    (nodelist_fp0 (reveal d.nodes))
+let dll_fp_f (#t:Type) (h0:heap) (d:dll t) : GTot Mod.loc =
+  let a = if is_null d.lhead then Mod.loc_none else Mod.loc_buffer (d.lhead^@h0).flink in
+  let b = if is_null d.ltail then Mod.loc_none else Mod.loc_buffer (d.ltail^@h0).flink in
+  Mod.loc_union // ghostly connections should give us this union for
+                // free, but still useful to have
+    (Mod.loc_union a b)
+    (nodelist_fp_f h0 (reveal d.nodes))
+let dll_fp_b (#t:Type) (h0:heap) (d:dll t) : GTot Mod.loc =
+  let a = if is_null d.lhead then Mod.loc_none else Mod.loc_buffer (d.lhead^@h0).blink in
+  let b = if is_null d.ltail then Mod.loc_none else Mod.loc_buffer (d.ltail^@h0).blink in
+  Mod.loc_union // ghostly connections should give us this union for
+                // free, but still useful to have
+    (Mod.loc_union a b)
+    (nodelist_fp_b h0 (reveal d.nodes))
+
+let piece_fp0 (#t:Type) (p:piece t) : GTot Mod.loc =
+  Mod.loc_union // ghostly connections should give us this union for
+                // free, but still useful to have
+    (Mod.loc_union (Mod.loc_buffer p.phead) (Mod.loc_buffer p.ptail))
+    (nodelist_fp0 (reveal p.pnodes))
+let piece_fp_f (#t:Type) (h0:heap) (p:piece t) : GTot Mod.loc =
+  Mod.loc_union // ghostly connections should give us this union for
+                // free, but still useful to have
+    (Mod.loc_union (Mod.loc_buffer (p.phead@h0).flink) (Mod.loc_buffer (p.ptail@h0).flink))
+    (nodelist_fp_f h0 (reveal p.pnodes))
+let piece_fp_b (#t:Type) (h0:heap) (p:piece t) : GTot Mod.loc =
+  Mod.loc_union // ghostly connections should give us this union for
+                // free, but still useful to have
+    (Mod.loc_union (Mod.loc_buffer (p.phead@h0).blink) (Mod.loc_buffer (p.ptail@h0).blink))
+    (nodelist_fp_b h0 (reveal p.pnodes))
+
 /// Anti aliasing properties
 
 (* TODO *)
